Naive LLVM memory interpretation
Does not support poison, nor non-int64 accesses

Veir/Interpreter/Basic.lean
@@ -1,3 +1,4 @@
+import Lean.Compiler
 import Veir.IR.Basic
 import Veir.Rewriter.Basic
 import Veir.ForLean
@@ -35,13 +36,50 @@ variable {OpInfo : Type} [HasOpInfo OpInfo]
 -/
 inductive RuntimeValue where
 | int (bitwidth : Nat) (value : LLVM.Int bitwidth)
+| addr (value : UInt64)
 | reg (value : RISCV.Reg)
 deriving Inhabited
 
 instance : ToString (RuntimeValue) where
   toString
     | .int _ val => ToString.toString val
+    | .addr val => ToString.toString val
     | .reg val => ToString.toString val
+
+structure MemoryState where
+  contents : ByteArray
+  size : UInt64
+
+def MemoryState.empty : MemoryState :=
+  { contents := ByteArray.emptyWithCapacity 1024, size := 8 }
+
+def MemoryState.alloc (state : MemoryState) (size : UInt64)
+    : MemoryState × UInt64 :=
+  ({contents := (ByteArray.empty.push 0).copySlice 0 state.contents (state.size + size).toNat 1, size := state.size + size}, state.size)
+
+def MemoryState.store (state : MemoryState) (addr : UInt64) (val : ByteArray)
+    : MemoryState :=
+  {state with contents := val.copySlice 0 state.contents addr.toNat val.size false}
+
+def MemoryState.storeValue (state : MemoryState) (addr : UInt64) (val : RuntimeValue)
+    : MemoryState :=
+  match val with
+  | .int 64 (.val v) | .reg {val := v} => state.store addr (Lean.Compiler.LCNF.uint64ToByteArrayLE v.toNat.toUInt64).toList.toByteArray
+  | .int _ .poison => state
+  | .addr v => state.store addr (Lean.Compiler.LCNF.uint64ToByteArrayLE v).toList.toByteArray
+  | _ => state
+
+def MemoryState.load (state : MemoryState) (addr size : UInt64)
+    : ByteArray :=
+  state.contents.extract addr.toNat (addr + size).toNat
+
+def MemoryState.loadValue (state : MemoryState) (addr : UInt64) (type : TypeAttr)
+    : Option RuntimeValue := do
+  match type.val with
+  | Attribute.integerType { bitwidth := 8 } => some (.int 8 (.val (BitVec.ofNat 8 (state.load addr 1)[0]!.toNat)))
+  | Attribute.integerType { bitwidth := 64 } => some (.int 64 (.val (BitVec.ofNat 64 (state.load 1 8).toUInt64LE!.toNat)))
+  --| Attribute.llvmPointerType _ => some (.addr (state.load addr 8).toUInt64LE!)
+  | _ => none
 
 /--
   The state of the interpreter at a given point in time.
@@ -49,6 +87,7 @@ instance : ToString (RuntimeValue) where
 -/
 structure InterpreterState where
   variables : Std.ExtHashMap ValuePtr RuntimeValue
+  memory : MemoryState
 
 /--
   Set the value of a variable.
@@ -67,6 +106,7 @@ def InterpreterState.getVar? (state : InterpreterState) (var : ValuePtr)
 @[ext]
 theorem InterpreterState.ext {s₁ s₂ : InterpreterState} :
     (∀ var, s₁.getVar? var = s₂.getVar? var) →
+    s₁.memory = s₂.memory →
     s₁ = s₂ := by
   rcases s₁; rcases s₂
   simp only [getVar?, mk.injEq]
@@ -116,7 +156,7 @@ def InterpreterState.setArgumentValues (state : InterpreterState) (ctx : IRConte
   Create an interpreter state with no variables defined.
 -/
 def InterpreterState.empty : InterpreterState :=
-  { variables := Std.ExtHashMap.emptyWithCapacity 8 }
+  { variables := Std.ExtHashMap.emptyWithCapacity 8, memory := .empty }
 
 /--
   How the control flow should proceed after interpreting a terminator.
@@ -299,28 +339,29 @@ def Arith.interpretOp' (opType : Veir.Arith) (properties : HasDialectOpInfo.prop
 
 def Llvm.interpretOp' (opType : Veir.Llvm) (properties : HasDialectOpInfo.propertiesOf opType)
     (resultTypes : Array TypeAttr) (operands : Array RuntimeValue) (blockOperands : Array BlockPtr)
-    : Interp ((Array RuntimeValue) × Option ControlFlowAction) :=
+    (mem : MemoryState)
+    : Interp ((Array RuntimeValue) × MemoryState × Option ControlFlowAction) :=
   match opType with
   | .mlir__constant => do
     let some resType := resultTypes[0]? | none
     let .integerType bw := resType.val
       | none
-    return (#[.int bw.bitwidth (LLVM.Int.constant bw.bitwidth properties.value.value)], none)
+    return (#[.int bw.bitwidth (LLVM.Int.constant bw.bitwidth properties.value.value)], mem, none)
   | .add => do
     let [.int bw lhs, .int bw' rhs] := operands.toList | none
     if h: bw' ≠ bw then none else
     let rhs := rhs.cast (by simp at h; exact h)
-    return (#[.int bw (LLVM.Int.add lhs rhs properties.nsw properties.nuw)], none)
+    return (#[.int bw (LLVM.Int.add lhs rhs properties.nsw properties.nuw)], mem, none)
   | .sub => do
     let [.int bw lhs, .int bw' rhs] := operands.toList | none
     if h: bw' ≠ bw then none else
     let rhs := rhs.cast (by simp at h; exact h)
-    return (#[.int bw (LLVM.Int.sub lhs rhs properties.nsw properties.nuw)], none)
+    return (#[.int bw (LLVM.Int.sub lhs rhs properties.nsw properties.nuw)], mem, none)
   | .mul => do
     let [.int bw lhs, .int bw' rhs] := operands.toList | none
     if h: bw' ≠ bw then none else
     let rhs := rhs.cast (by simp at h; exact h)
-    return (#[.int bw (LLVM.Int.mul lhs rhs properties.nsw properties.nuw)], none)
+    return (#[.int bw (LLVM.Int.mul lhs rhs properties.nsw properties.nuw)], mem, none)
   | .sdiv => do
     let [.int bw lhs, .int bw' rhs] := operands.toList | none
     if h: bw' ≠ bw then none else
@@ -334,9 +375,9 @@ def Llvm.interpretOp' (opType : Veir.Llvm) (properties : HasDialectOpInfo.proper
         | .poison => Interp.ub
         | .val v =>
           if v = BitVec.intMin bw then Interp.ub
-          else return (#[.int bw (LLVM.Int.sdiv lhs rhs properties.exact)], none)
+          else return (#[.int bw (LLVM.Int.sdiv lhs rhs properties.exact)], mem, none)
       else
-        return (#[.int bw (LLVM.Int.sdiv lhs rhs properties.exact)], none)
+        return (#[.int bw (LLVM.Int.sdiv lhs rhs properties.exact)], mem, none)
   | .udiv => do
     let [.int bw lhs, .int bw' rhs] := operands.toList | none
     if h: bw' ≠ bw then none else
@@ -345,7 +386,7 @@ def Llvm.interpretOp' (opType : Veir.Llvm) (properties : HasDialectOpInfo.proper
     | .poison => Interp.ub
     | .val v' =>
       if v' = 0 then Interp.ub
-      else return (#[.int bw (LLVM.Int.udiv lhs rhs properties.exact)], none)
+      else return (#[.int bw (LLVM.Int.udiv lhs rhs properties.exact)], mem, none)
   | .srem => do
     let [.int bw lhs, .int bw' rhs] := operands.toList | none
     if h: bw' ≠ bw then none else
@@ -359,9 +400,9 @@ def Llvm.interpretOp' (opType : Veir.Llvm) (properties : HasDialectOpInfo.proper
         | .poison => Interp.ub
         | .val v =>
           if v = BitVec.intMin bw then Interp.ub
-          else return (#[.int bw (LLVM.Int.srem lhs rhs)], none)
+          else return (#[.int bw (LLVM.Int.srem lhs rhs)], mem, none)
       else
-        return (#[.int bw (LLVM.Int.srem lhs rhs)], none)
+        return (#[.int bw (LLVM.Int.srem lhs rhs)], mem, none)
   | .urem => do
     let [.int bw lhs, .int bw' rhs] := operands.toList | none
     if h: bw' ≠ bw then none else
@@ -370,71 +411,71 @@ def Llvm.interpretOp' (opType : Veir.Llvm) (properties : HasDialectOpInfo.proper
     | .poison => Interp.ub
     | .val v' =>
       if v' = 0 then Interp.ub
-      else return (#[.int bw (LLVM.Int.urem lhs rhs)], none)
+      else return (#[.int bw (LLVM.Int.urem lhs rhs)], mem, none)
   | .shl => do
     let [.int bw lhs, .int bw' rhs] := operands.toList | none
     if h: bw' ≠ bw then none else
     let rhs := rhs.cast (by simp at h; exact h)
-    return (#[.int bw (LLVM.Int.shl lhs rhs properties.nsw properties.nuw)], none)
+    return (#[.int bw (LLVM.Int.shl lhs rhs properties.nsw properties.nuw)], mem, none)
   | .lshr => do
     let [.int bw lhs, .int bw' rhs] := operands.toList | none
     if h: bw' ≠ bw then none else
     let rhs := rhs.cast (by simp at h; exact h)
-    return (#[.int bw (LLVM.Int.lshr lhs rhs properties.exact)], none)
+    return (#[.int bw (LLVM.Int.lshr lhs rhs properties.exact)], mem, none)
   | .ashr => do
     let [.int bw lhs, .int bw' rhs] := operands.toList | none
     if h: bw' ≠ bw then none else
     let rhs := rhs.cast (by simp at h; exact h)
-    return (#[.int bw (LLVM.Int.ashr lhs rhs properties.exact)], none)
+    return (#[.int bw (LLVM.Int.ashr lhs rhs properties.exact)], mem, none)
   | .and => do
     let [.int bw lhs, .int bw' rhs] := operands.toList | none
     if h: bw' ≠ bw then none else
     let rhs := rhs.cast (by simp at h; exact h)
-    return (#[.int bw (LLVM.Int.and lhs rhs)], none)
+    return (#[.int bw (LLVM.Int.and lhs rhs)], mem, none)
   | .or => do
     let [.int bw lhs, .int bw' rhs] := operands.toList | none
     if h: bw' ≠ bw then none else
     let rhs := rhs.cast (by simp at h; exact h)
-    return (#[.int bw (LLVM.Int.or lhs rhs properties.disjoint)], none)
+    return (#[.int bw (LLVM.Int.or lhs rhs properties.disjoint)], mem, none)
   | .xor => do
     let [.int bw lhs, .int bw' rhs] := operands.toList | none
     if h: bw' ≠ bw then none else
     let rhs := rhs.cast (by simp at h; exact h)
-    return (#[.int bw (LLVM.Int.xor lhs rhs)], none)
+    return (#[.int bw (LLVM.Int.xor lhs rhs)], mem, none)
   | .trunc => do
     let [.int w val] := operands.toList | none
     let some resType := resultTypes[0]? | none
     let .integerType resBw := resType.val | none
     if h: resBw.bitwidth >= w then none else
-    return (#[.int resBw.bitwidth (LLVM.Int.trunc val resBw.bitwidth properties.nsw properties.nuw (by omega))], none)
+    return (#[.int resBw.bitwidth (LLVM.Int.trunc val resBw.bitwidth properties.nsw properties.nuw (by omega))], mem, none)
   | .zext => do
     let [.int w val] := operands.toList | none
     let some resType := resultTypes[0]? | none
     let .integerType resBw := resType.val | none
     if h: resBw.bitwidth <= w then none else
-    return (#[.int resBw.bitwidth (LLVM.Int.zext val resBw.bitwidth properties.nneg (by omega))], none)
+    return (#[.int resBw.bitwidth (LLVM.Int.zext val resBw.bitwidth properties.nneg (by omega))], mem, none)
   | .sext => do
     let [.int w val] := operands.toList | none
     let some resType := resultTypes[0]? | none
     let .integerType resBw := resType.val | none
     if h: resBw.bitwidth <= w then none else
-    return (#[.int resBw.bitwidth (LLVM.Int.sext val resBw.bitwidth (by omega))], none)
+    return (#[.int resBw.bitwidth (LLVM.Int.sext val resBw.bitwidth (by omega))], mem, none)
   | .icmp => do
     let [.int bw lhs, .int bw' rhs] := operands.toList | none
     if h: bw' ≠ bw then none else
     let rhs := rhs.cast (by simpa using h)
     let some p := LLVM.IntPred.fromNat properties.value.value.toNat | none
-    return (#[.int 1 (LLVM.Int.icmp lhs rhs p)], none)
+    return (#[.int 1 (LLVM.Int.icmp lhs rhs p)], mem, none)
   | .select => do
     let [.int 1 cond, .int bw lhs, .int bw' rhs] := operands.toList | none
     if h: bw' ≠ bw then none else
     let rhs := rhs.cast (by simpa using h)
-    return (#[.int bw (LLVM.Int.select cond lhs rhs)], none)
+    return (#[.int bw (LLVM.Int.select cond lhs rhs)], mem, none)
   | .return => do
-    return (#[], some (.return operands))
+    return (#[], mem, some (.return operands))
   | .br => do
     let [dest] := blockOperands.toList | none
-    return (#[], some (.branch operands dest))
+    return (#[], mem, some (.branch operands dest))
   | .cond_br => do
     let [destTrue, destFalse] := blockOperands.toList | none
     let some condVal := operands[0]? | none
@@ -443,11 +484,29 @@ def Llvm.interpretOp' (opType : Veir.Llvm) (properties : HasDialectOpInfo.proper
     match condVal with
     | .int 1 (.val cond) =>
       if cond = 1#1 then
-        return (#[], some (.branch (operands.extract 1 (trueSize + 1)) destTrue))
+        return (#[], mem, some (.branch (operands.extract 1 (trueSize + 1)) destTrue))
       else
-        return (#[], some (.branch (operands.extract (trueSize + 1) operands.size) destFalse))
+        return (#[], mem, some (.branch (operands.extract (trueSize + 1) operands.size) destFalse))
     | .int 1 .poison => Interp.ub
     | _ => none
+  | .alloca => do
+    let [.int _ (.val count)] := operands.toList | none
+    let size ← match properties.elem_type.val with
+    | Attribute.integerType { bitwidth := bw } => some (.ok (bw / 8))
+    | .llvmPointerType _ => some (.ok 8)
+    | _ => none
+    let totalSize := (size * count.toNat).toUInt64
+    let (mem, addr) := mem.alloc totalSize
+    return (#[.addr addr], mem, none)
+  | load => do
+    let [.addr addr] := operands.toList | none
+    let [type] := resultTypes.toList | none
+    let val ← mem.loadValue addr type
+    return (#[val], mem, none)
+  | .store => do
+    let [.addr addr, val] := operands.toList | none
+    let mem := mem.storeValue addr val
+    return (#[], mem, none)
   | _ => none
 
 def Riscv.interpretOp' (opType : Veir.Riscv) (properties : HasDialectOpInfo.propertiesOf opType)
@@ -822,30 +881,36 @@ def HW.interpretOp' (opType : Veir.HW) (properties : HasDialectOpInfo.properties
 -/
 def interpretOp' (opType : OpCode) (properties : HasOpInfo.propertiesOf opType)
     (resultTypes : Array TypeAttr) (operands : Array RuntimeValue) (blockOperands : Array BlockPtr)
-    : Interp ((Array RuntimeValue) × Option ControlFlowAction) :=
+    (mem : MemoryState)
+    : Interp ((Array RuntimeValue) × MemoryState × Option ControlFlowAction) :=
   match opType with
   | .arith arithOp => do
-    Arith.interpretOp' arithOp properties resultTypes operands blockOperands
+    let (vals, act) ← Arith.interpretOp' arithOp properties resultTypes operands blockOperands
+    return (vals, mem, act)
   | .llvm llvmOp => do
-    Llvm.interpretOp' llvmOp properties resultTypes operands blockOperands
+    Llvm.interpretOp' llvmOp properties resultTypes operands blockOperands mem
   | .riscv riscvOp => do
-    Riscv.interpretOp' riscvOp properties resultTypes operands blockOperands
+    let (vals, act) ← Riscv.interpretOp' riscvOp properties resultTypes operands blockOperands
+    return (vals, mem, act)
   | .cf cfOp => do
-    Cf.interpretOp' cfOp properties resultTypes operands blockOperands
+    let (vals, act) ← Cf.interpretOp' cfOp properties resultTypes operands blockOperands
+    return (vals, mem, act)
   | .comb combOp => do
-    Comb.interpretOp' combOp properties operands blockOperands
+    let (vals, act) ← Comb.interpretOp' combOp properties operands blockOperands
+    return (vals, mem, act)
   | .hw hwOp => do
-    HW.interpretOp' hwOp properties resultTypes blockOperands
+    let (vals, act) ← HW.interpretOp' hwOp properties resultTypes blockOperands
+    return (vals, mem, act)
   | .func .return => do
-    return (#[], some (.return operands))
+    return (#[], mem, some (.return operands))
   | .builtin .unrealized_conversion_cast => do
     let some resType := resultTypes[0]? | none
     match resType.val, operands.toList with
     | .registerType _, [.int _bw val] =>
-      return (#[.reg (LLVM.Int.toReg val )], none)
+      return (#[.reg (LLVM.Int.toReg val )], mem, none)
     | .integerType _bw, [.reg val] =>
       let .integerType resBw := resType.val | none
-      return (#[.int resBw.bitwidth (RISCV.Reg.toInt val resBw.bitwidth)], none)
+      return (#[.int resBw.bitwidth (RISCV.Reg.toInt val resBw.bitwidth)], mem, none)
     | _ , _ => none
   | _ => none
 
@@ -860,8 +925,8 @@ def interpretOp (ctx : IRContext OpCode) (op : OperationPtr) (state : Interprete
     : Interp (InterpreterState × Option ControlFlowAction) := do
   let some operands := state.getOperandValues ctx op | none
   let opType := op.getOpType! ctx
-  let (resultValues, action) ← interpretOp' opType (op.getProperties! ctx opType) (op.getResultTypes! ctx) operands (op.getSuccessors! ctx)
-  let newState := state.setResultValues ctx op resultValues
+  let (resultValues, mem, action) ← interpretOp' opType (op.getProperties! ctx opType) (op.getResultTypes! ctx) operands (op.getSuccessors! ctx) state.memory
+  let newState := {state.setResultValues ctx op resultValues with memory := mem}
   return (newState, action)
 
 /--
