Test/Interpreter/LLVM/mem.mlir
@@ -1,0 +1,12 @@
+// RUN: veir-interpret %s | filecheck %s
+
+"builtin.module"() ({
+  %1 = "llvm.constant"() <{ "value" = 1 : i64 }> : () -> i64
+  %2 = "llvm.constant"() <{ "value" = 8 : i64 }> : () -> i64
+  %3 = "llvm.alloca"(%1) <{ "elem_type" = i64 }> : (i64) -> !llvm.ptr
+  "llvm.store"(%3, %2) : (!llvm.ptr, i64) -> ()
+  %4 = "llvm.load"(%3) : (!llvm.ptr) -> i64
+  "func.return"(%4) : (i64) -> ()
+}) : () -> ()
+
+// CHECK: Program output: #[0x00000008#32]
